proof/refine/RISCV64/Invariants_H.thy
@@ -842,24 +842,16 @@ definition sch_act_sane :: "kernel_state \<Rightarrow> bool" where
 abbreviation
   "sch_act_not t \<equiv> \<lambda>s. ksSchedulerAction s \<noteq> SwitchToThread t"
 
-definition
-  idle_tcb'_2 :: "Structures_H.thread_state \<times> machine_word option \<Rightarrow> bool"
-where
-  "idle_tcb'_2 \<equiv> \<lambda>(st, ntfn_opt).
-                    (idle' st \<and> ntfn_opt = None)"
+definition idle_tcb'_2 :: "Structures_H.thread_state \<times> machine_word option \<Rightarrow> bool" where
+  "idle_tcb'_2 \<equiv> \<lambda>(st, ntfn_opt). (idle' st \<and> ntfn_opt = None)"
 
 abbreviation
-  "idle_tcb' tcb \<equiv>
-      idle_tcb'_2 (tcbState tcb, tcbBoundNotification tcb)"
+  "idle_tcb' tcb \<equiv> idle_tcb'_2 (tcbState tcb, tcbBoundNotification tcb)"
 
 lemmas idle_tcb'_def = idle_tcb'_2_def
 
-definition
-  valid_idle' :: "kernel_state \<Rightarrow> bool"
-where
-  "valid_idle' \<equiv>
-     \<lambda>s. obj_at' idle_tcb' (ksIdleThread s) s
-         \<and> idle_thread_ptr = ksIdleThread s"
+definition valid_idle' :: "kernel_state \<Rightarrow> bool" where
+  "valid_idle' \<equiv> \<lambda>s. obj_at' idle_tcb' (ksIdleThread s) s \<and> idle_thread_ptr = ksIdleThread s"
 
 lemma valid_idle'_tcb_at':
   "valid_idle' s \<Longrightarrow> obj_at' idle_tcb' (ksIdleThread s) s"
